\documentclass[11pt, oneside]{article}   	% use "amsart" instead of "article" for AMSLaTeX format
\usepackage{geometry}                		% See geometry.pdf to learn the layout options. There are lots.
\geometry{letterpaper}                   		% ... or a4paper or a5paper or ... 
%\geometry{landscape}                		% Activate for rotated page geometry
%\usepackage[parfill]{parskip}    		% Activate to begin paragraphs with an empty line rather than an indent
\usepackage{graphicx}				% Use pdf, png, jpg, or epsÂ§ with pdflatex; use eps in DVI mode
								% TeX will automatically convert eps --> pdf in pdflatex		
\usepackage{amssymb}

%SetFonts

%SetFonts


\title{Assignment 2 Problem 2}
\author{Michael Cai}
\date{\today}							% Activate to display a given date or no date

\begin{document}
\maketitle

\noindent \textbf{2.} \textit{Let $K_m$ denote the following indefinite integral:}\\
$K_m(x) = \int_ x^m sin(x)dx$ for $m = 0,1,2...$\\~\\
(a) \textit{Evaluate $K_1(x)$}. \\
$K_1(x) = \int x^1 sin(x)dx$\\
Integration by parts would be the strategy to solve the integral because the integrand is a product. Therefore, we let $u = x$ and thus $du = dx$ and $dv = sinxdx$ and thus $v = -cosx$.\\
$\int x^1 sin(x) = -xcosx + \int cosxdx$ \\
$ = -xcosx + sinx + C$\\

\noindent (b) \textit {Show $K_m(x) = -x^m cos(x) + mx^{m-1}sin(x) - m(m-1)K_{m-2}x$}\\
$K_m(x) = \int x^m sin(x)dx$\\
Because the integrand is a product, I am going to use integration by parts and select $u = x^m$ and thus $du = mx^{m-1}dx$. I choose $dv = sin(x)dx$ and thus $v = -cos(x)$. \\
Therefore $\int x^msin(x)dx = -x^mcos(x) + \int mx^{m-1}cos(x)dx$\\~\\
Now consider $\int mx^{m-1}cos(x)dx$ which equals $m \int x^{m-1}cos(x)dx$\\
Again we use integration by parts because the integrand is a product.\\
I choose $u = x^{m-1}$ and thus $du = (m-1)x^{m-2}dx$. I choose $dv = cos(x)dx$ and thus $v = sin(x)$.\\
Therefore $m \int x^{m-1} cos(x)dx = m(x^{m-1}sin(x) - (m-1) \int x^{m-2}sin(x)dx$\\
$= mx^{m-1}sin(x)-m(m-1) \int x^{m-2} sin(x)dx$\\
This last integral $\int x^{m-2} sin(x)dx$ is equal to $K_{m-2}(x)$. \\~\\
Thus, plugging this integral back into the original equation, where we left off: \\
$\int x^msin(x)dx = -x^mcos(x) + \int mx^{m-1}cos(x)dx$\\
$= \int x^msin(x)dx = -x^mcos(x) + mx^{m-1}sin(x)-m(m-1) K_{m-2}(x)$\\~\\~\\

\noindent (c) \textit{ Calculate $K_0(x)$, $K_2(x)$, and $K_4(x)$}\\
$K_0(x) = \int x^0 sin(x)dx = \int sin(x)dx = -cos(x) + C$\\
$K_2(x) = \int x^2sin(x)dx$\\
Because the integrand is a product, we again apply integration by parts.\\
I choose $u = x^2$ and thus $du = 2xdx$. I choose $dv = sin(x)dx$ and thus $v = -cos(x)$.\\
Therefore $\int x^2 sin(x)dx = -x^2cos(x) + 2 \int xcos(x)dx$.\\
Consider the integral $\int xcos(x)dx$\\
Again we apply IBP. Let $u = x$ and thus $du = dx$. Let $dv = cos(x)dx$ and thus $v = sin(x)$.\\
$\int xcos(x)dx = xsin(x) - \int sin(x)dx = xsin(x) - cos(x) + C$\\~\\
Plugging this back into the original equations we get:\\
$\int x^2 sin(x)dx = -x^2cos(x) + 2 \int xcos(x)dx = -x^2cos(x) + 2(xsin(x) - cos(x) + C)$\\
$= -x^2cos(x) + 2xsin(x) + 2cos(x) + C': C' = 2C$\\~\\
$K_4(x) = \int x^4 sin(x)dx$\\
Recall the formula for $K_m(x)$:\\
$\int x^msin(x)dx = -x^mcos(x) + mx^{m-1}sin(x)-m(m-1) K_{m-2}(x)$\\
Thus we choose m = 4 and we get:\\
$= \int x^4sin(x)dx = -x^4cos(x) + 4x^3 sin(x) - 4(3)K_2(x)$\\
Then we plug in $K_2(x)$ and we get:\\
$= -x^4cos(x) + 4x^3sin(x) + 12x^2cos(x) + 24xsin(x) + 24cos(x) + C$\\

\noindent(d) \textit{Solve the definite integral $\int_0^\pi x^4 sin(x)dx$}\\
To get the answer, we just need to evaluate the indefinite integral that we just calculated with the bounds 0 and $\pi$. \\
$\int_0^\pi x^4 sin(x)dx$ equals\\
$-\pi^4cos(\pi) + 4\pi^3sin(\pi) + 12\pi^2cos(\pi) + 24\pi sin(\pi) + 24cos(\pi)$\\
minus $(0^4cos(0) + 4(0)^3sin(0) + 12(0)^2cos(0) + 24(0) sin(0) + 24cos(0))$\\
$= \pi^4 - 12\pi^2 - 24 - 24 = \pi^4 - 12\pi^2 - 48$.\\




\end{document}  