\documentclass[11pt, oneside]{article}   	% use "amsart" instead of "article" for AMSLaTeX format
\usepackage{geometry}                		% See geometry.pdf to learn the layout options. There are lots.
\geometry{letterpaper}                   		% ... or a4paper or a5paper or ... 
%\geometry{landscape}                		% Activate for rotated page geometry
%\usepackage[parfill]{parskip}    		% Activate to begin paragraphs with an empty line rather than an indent
\usepackage{graphicx}				% Use pdf, png, jpg, or epsÂ§ with pdflatex; use eps in DVI mode
								% TeX will automatically convert eps --> pdf in pdflatex		
\usepackage{amssymb}

%SetFonts

%SetFonts


\title{Assignment 2 Problem 3}
\author{Michael Cai}
\date{\today}							% Activate to display a given date or no date

\begin{document}
\maketitle

\noindent3. \\
(a)
\textit{Use the formulas for $sin(A+B)$ and $sin(A-B)$ to show that:}\\
$sinAcosB = \frac{1}{2}[sin(A-B) + sin(A+B)]$\\~\\
The Angle Addition Identity for $sin$ states:\\
$sin(A+B) = sinAcosB + cosAsinB$\\
$sin(A-B) = sinAcosB - cosAsinB$\\~\\
Prove: $sinAcosB = \frac{1}{2}[sin(A-B) + sin(A+B)$\\~\\
$sin(A+B) = sinAcosB + cosAsinB$\\
$sinAcosB = sin(A+B) - cosAsinB$\\
Now add $sin(A-B)$ to both sides\\
$sinAcosB + sin(A-B) = sin(A+B) -cosAsinB + sin(A-B)$\\
Expand on the left hand side\\
$sinAcosB + sinAcosB - cosAsinB = sin(A=B) +sin(A+B) - cosAsinB$\\
$2sinAcosB - cosAsinB + cosAsinB = sin(A-B) + sin(A+B)$\\~\\
Therefore $sinAcosB = \frac{1}{2}(sin(A-B) + sin(A+B))$\\

\noindent (b) \textit{Use part (a) to evaluate $\int sin(3x)cos(x)dx$}\\
Recall from part (a) that $sinAcosB = \frac{1}{2}(sin(A-B) + sin(A+B))$\\
Plug it in:\\
$\int sin(3x)cos(x)dx = \frac{1}{2}(sin(3x-x) + sin(3x+x))$\\
$= \frac{1}{2} \int sin(2x) + sin(4x)dx$\\
$= \frac{1}{2} \int sin(2x)dx + \frac{1}{2} \int sin(4x)dx$\\~\\
First consider $\int sin(2x)dx$:\\
By the double angle formula, $\int sin(2x)dx = \int 2sinxcosx dx$\\
Therefore, we I use u-substitution on $\in 2sinxcosx dx$ and set $u = sinx$ making $du = cosxdx$.\\
Thus $\int 2sinxcosx = 2 \int udu = 2 (\frac{1}{2} u^2 + C) = u^2 + C = sin^2(x) + C$\\~\\

\noindent Now we consider $\int sin(4x)dx$:\\
Also apply the double angle formula.\\
$\int sin(4x)dx = \int sin(2(2x))dx = \int 2sin(2x)cos(2x)dx$\\
If you expand both the sin(2x) and cos(2x) components of this new integral using the double angle formula you get:\\
$2 \int (2sin(x)cos(x))(cos^2(x)-sin^2(x)) dx$\\
$= 2 \int 2sinxcos^3(x) - 2 sin^3(x)cos(x) dx$\\
$= 4 \int cos^3(x) sin(x)dx - 4 \int sin^3(x)cos(x)dx$\\~\\
Now we use u-substitution for both integrals ($u$ for the first and $u'$ for the second)\\
Let $u = cos(x)$ and thus $du = -sin(x)dx$. \\
Let $u' = sin(x)$ and thus $du' = cos(x)dx$. \\~\\
Therefore, $4 \int cos^3(x) sin(x)dx - 4 \int sin^3(x)cos(x)dx = 4 \int u^3 du - 4 \int u'^3 du'$\\
$= -4(\frac{1}{4}u^4 + C) -4(\frac{1}{4}u'^4+C')$\\
$= -cos^4(x) - sin^4(x) + C''$\\~\\
Plugging it all back together we get:\\
$\int sin(3x)cos(x)dx = \frac{1}{2}(sin(2x) + sin(4x))$\\
$= \frac{1}{2}(-cos^4(x) - sin^4(x) + C'') + \frac{1}{2}(sin^2(x)+C)$\\
$= -\frac{1}{2}cos^4(x)-\frac{1}{2}sin^4(x) + \frac{1}{2}sin^2(x) + C$


\end{document}  